Broke CG into multiple modules.

src/CG.v
@@ -1,5 +1,9 @@
 Require Import Coq.Lists.List.
 Require Import Coq.Relations.Relation_Definitions.
+Require Import Coq.Lists.ListSet.
+Require Import Aniceto.ListSet.
+Require Import Aniceto.Graphs.Graph.
+
 Require Import HJ.Tid.
 Require Import HJ.Mid.
 Require Import HJ.Cid.
@@ -32,7 +36,7 @@ Module Node.
 End Node.
 
 Module Trace.
-  Inductive op_type := SPAWN | JOIN.
+  Inductive op_type := FORK | JOIN.
 
   Structure op := {
     op_t: op_type;
@@ -40,16 +44,8 @@ Module Trace.
     op_dst: tid
   }.
 
-  Definition trace := list (option op).
+  Definition trace := list op.
 
-  Definition from_effect (e:Lang.effect) :=
-  match e with
-  | (x, Lang.FUTURE y) => Some {|op_t:=SPAWN; op_src:=x; op_dst:=y|}
-  | (x, Lang.FORCE y) => Some {|op_t:=JOIN; op_src:=x; op_dst:=y|}
-  | _ => None
-  end.
-
-  Definition from_effects := map from_effect.
 End Trace.
 
 Section CG.
@@ -72,13 +68,13 @@ Section Defs.
   }.
 
   Inductive Check : tee -> Prop :=
-  | check_spawn:
+  | check_fork:
     forall x y dx last_id,
     dx < last_id ->
     x <> y ->
     Check
     {|
-      ntype := SPAWN;
+      ntype := FORK;
       intra :=
       (
         {| node_task := x; node_dag_id := dx |},
@@ -115,9 +111,9 @@ Section Defs.
   Definition tee_last_id (t:tee) :=
   node_dag_id (snd (inter t)).
 
-  Definition mk_spawn last_id (x:node) y :=
+  Definition mk_fork last_id (x:node) y :=
   {|
-    ntype := SPAWN;
+    ntype := FORK;
     intra := (x, {| node_task := (node_task x); node_dag_id := S last_id |} );
     inter := (x, {| node_task := y; node_dag_id := S (S last_id) |})
   |}.
@@ -144,10 +140,10 @@ Section Defs.
     inversion H; simpl in *; auto.
   Qed.
 
-  Lemma check_inter_dag_spawn:
+  Lemma check_inter_dag_fork:
     forall v,
     Check v ->
-    ntype v = SPAWN ->
+    ntype v = FORK ->
     fst (intra v) = fst (inter v).
   Proof.
     intros.
@@ -189,10 +185,10 @@ Section Defs.
     inversion H; simpl in *; auto.
   Qed.
 
-  Lemma check_dag_lt_spawn:
+  Lemma check_dag_lt_fork:
     forall v,
     Check v ->
-    ntype v = SPAWN ->
+    ntype v = FORK ->
     dag_lt (snd (intra v)) (snd (inter v)).
   Proof.
     intros.
@@ -236,16 +232,16 @@ Section Defs.
 
   Definition cg_nodes_add (t:tee) (m: MT.t node) :=
   match t with
-  | {| ntype := SPAWN; intra:=(_,x); inter:=(_,y) |} =>
+  | {| ntype := FORK; intra:=(_,x); inter:=(_,y) |} =>
     (MT.add (node_task x) x)
     (MT.add (node_task y) y m)
   | {| ntype := JOIN; intra:=(_,x); inter:=_ |} => 
     MT.add (node_task x) x m
   end.
 
-  Definition tee_spawn (x y:tid) (cg : computation_graph) : option tee :=
+  Definition tee_fork (x y:tid) (cg : computation_graph) : option tee :=
   match cg_lookup x cg with
-  | Some nx => Some (mk_spawn (cg_last_id cg) nx y)
+  | Some nx => Some (mk_fork (cg_last_id cg) nx y)
   | _ => None
   end.
 
@@ -255,118 +251,252 @@ Section Defs.
   | _ => None
   end.
 
-  Definition cg_add (v:tee) (cg : computation_graph) : computation_graph :=
+  Definition cg_add (o:option tee) (cg : computation_graph) : computation_graph :=
+  match o with
+  | Some v =>
     {| cg_tees := v :: cg_tees cg;
        cg_last_id := (tee_last_id v);
-       cg_nodes := cg_nodes_add v (cg_nodes cg) |}.
+       cg_nodes := cg_nodes_add v (cg_nodes cg) |}
+  | None => cg
+  end.
 
-  Definition tee_eval o : computation_graph -> option tee :=
+  Definition cg_fork (x y:tid) (cg : computation_graph) : computation_graph :=
+  cg_add (tee_fork x y cg) cg.
+
+  Definition cg_join (x y:tid) (cg : computation_graph) : computation_graph :=
+  cg_add (tee_join x y cg) cg.
+
+  Definition cg_eval (o:op) cg :=
   match o with
   | {| op_t := e; op_src := x; op_dst := y |} =>
     let f := (match e with
-    | SPAWN => tee_spawn
-    | JOIN => tee_join
-    end) in
-    f x y
-  end.
-
-  Definition cg_eval (o:option op) cg :=
-  match o with
-  | Some o =>
-    match (tee_eval o cg) with
-    | Some v => cg_add v cg
-    | _ => cg
-    end
-  | None => cg
+      | FORK => cg_fork
+      | JOIN => cg_join
+      end)
+    in
+    f x y cg
   end.
 
   (** Compute a CG from a trace. *)
 
-  Definition trace_to_cg (x:tid) ts := fold_left (fun cg o => cg_eval o cg) ts (make_cg x).
-
-  (** Compute a CG from a trace of our language. *)
-
-  Definition effects_to_cg (x:tid) ts := trace_to_cg x (from_effects ts).
+  Fixpoint trace_to_cg (x:tid) l := 
+  match l with
+  | (o::l) => cg_eval o (trace_to_cg x l)
+  | nil => make_cg x
+  end.
 
   Inductive Lookup t n cg: Prop :=
   | lookup_def: 
     MT.MapsTo t n (cg_nodes cg) ->
     Lookup t n cg.
 
-  Inductive CG: trace -> computation_graph -> Prop :=
+  Definition In (t:tid) cg := MT.In t (cg_nodes cg).
+
+  Lemma in_make:
+    forall t,
+    In t (make_cg t).
+  Proof.
+    intros.
+    unfold make_cg, In.
+    simpl.
+    rewrite MT_Facts.add_in_iff.
+    auto.
+  Qed.
+
+  Let tee_fork_inv_some:
+    forall x y t cg,
+    tee_fork x y cg = Some t ->
+    exists n, MT.MapsTo x n (cg_nodes cg) /\ t = mk_fork (cg_last_id cg) n y.
+  Proof.
+    unfold tee_fork, cg_lookup.
+    intros.
+    destruct (MT_Extra.find_rw x (cg_nodes cg)) as [(R,?)|(n,(R,?))];
+    rewrite R in *; clear R; inversion H.
+    eauto.
+  Qed.
+
+  Let tee_fork_inv_none:
+    forall x y cg,
+    tee_fork x y cg = None ->
+    ~ MT.In x (cg_nodes cg).
+  Proof.
+    unfold tee_fork, cg_lookup.
+    intros.
+    destruct (MT_Extra.find_rw x (cg_nodes cg)) as [(R,?)|(n,(R,?))];
+    rewrite R in *; clear R; inversion H.
+    eauto.
+  Qed.
+
+  Lemma in_fork_1:
+    forall x y cg,
+    In x cg ->
+    In y (cg_fork x y cg).
+  Proof.
+    intros.
+    unfold cg_fork, In, cg_add.
+    destruct cg.
+    remember (tee_fork _ _ _).
+    symmetry in Heqo.
+    destruct o; simpl in *.
+    - apply tee_fork_inv_some in Heqo.
+      destruct Heqo as (n, (mt, R)).
+      subst.
+      simpl in *.
+      rewrite MT_Facts.add_in_iff.
+      right.
+      rewrite MT_Facts.add_in_iff; auto.
+    - apply tee_fork_inv_none in Heqo.
+      contradiction.
+  Qed.
+
+  Let in_cg_add:
+    forall z cg o,
+    MT.In z (cg_nodes cg) ->
+    MT.In z (cg_nodes (cg_add o cg)).
+  Proof.
+    unfold cg_add, cg_nodes_add.
+    destruct cg, o; simpl in *; intros.
+    - destruct t; destruct ntype0, intra0, inter0; simpl;
+      repeat rewrite MT_Facts.add_in_iff; auto.
+    - auto.
+  Qed.
+
+
+  Lemma in_fork_2:
+    forall x y z cg,
+    In z cg ->
+    In z (cg_fork x y cg).
+  Proof.
+    unfold cg_fork, In.
+    intros.
+    auto.
+  Qed.
+
+  Lemma in_join_2:
+    forall x y z cg,
+    In z cg ->
+    In z (cg_join x y cg).
+  Proof.
+    unfold cg_join, In.
+    intros.
+    auto.
+  Qed.
+
+  Inductive CG (x:tid): trace -> computation_graph -> Prop :=
   | cg_nil:
-    forall x,
-    CG nil (make_cg x)
-  | cg_cons:
-    forall o l cg,
-    CG l cg ->
-    CG (o::l) (cg_eval o cg).
+    CG x nil (make_cg x)
+  | cg_cons_fork:
+    forall a b l cg,
+    CG x l cg ->
+    In a cg ->
+    CG x ({| op_t := FORK; op_src := a; op_dst := b |} :: l) (cg_fork a b cg)
+  | cg_cons_join:
+    forall a b l cg,
+    CG x l cg ->
+    In a cg ->
+    In b cg ->
+    CG x ({| op_t := JOIN; op_src := a; op_dst := b |} :: l) (cg_join a b cg).
 
-  Definition is_evt (o:Lang.op) :=
-  match o with
-  | Lang.FUTURE _ => true
-  | Lang.FORCE _ => true
-  | _ => false
-  end.
-
-
-  Inductive Reduces: computation_graph -> Lang.effect -> computation_graph -> Prop :=
-  | reduces_def:
-    forall cg e,
-    Reduces cg e (cg_eval (from_effect e) cg).
+  Lemma cg_fun:
+    forall x l cg cg',
+    CG x l cg ->
+    CG x l cg' ->
+    cg = cg'.
+  Proof.
+    induction l; intros. {
+      inversion H; inversion H0; auto.
+    }
+    destruct a;
+    destruct op_t0;
+    inversion H;
+    inversion H0;
+    subst;
+    assert (cg0 = cg1) by auto; subst; auto.
+  Qed.
 
   (**
     Ensure the names are being used properly; no continue edges after a task
     has been termianted (target of a join).
     *)
 
-  Inductive Continue v : edge -> Prop :=
-    continue_def:
-      Continue v (intra v).
+  Inductive edge_type :=
+  | CONTINUE_EDGE
+  | FORK_EDGE
+  | JOIN_EDGE.
 
-  Inductive Spawn: tee -> edge -> Prop :=
-    spawn_def:
-      forall v,
-      ntype v = SPAWN ->
-      Spawn v (inter v).
+  Inductive Edge : edge_type -> edge -> tee -> Prop :=
+  | edge_continue:
+    forall t,
+    Edge CONTINUE_EDGE (intra t) t
+  | edge_fork:
+    forall t,
+    Edge FORK_EDGE (inter t) t
+  | edge_join:
+    forall t,
+    Edge JOIN_EDGE (inter t) t.
 
-  Inductive Join: tee -> edge -> Prop :=
-    join_def:
-      forall v,
-      ntype v = JOIN ->
-      Join v (inter v).
-
-  Inductive Prec t e : Prop :=
-  | prec_continue:
-    Continue t e ->
-    Prec t e
-  | prec_spawn:
-    Spawn t e ->
-    Prec t e
-  | prec_join:
-    Join t e ->
-    Prec t e.
-
-  Inductive ListEdge {A:Type} {B:Type} P l (e:B*B) : Prop :=
-  | list_edge_def:
-    forall (x:A),
-    List.In x l ->
-    P x e ->
-    ListEdge P l e.
-
-  Let LContinue := ListEdge Continue.
-  Let LSpawn := ListEdge Spawn.
-  Let LPrec := ListEdge Prec.
-
-  Require Import Aniceto.Graphs.Graph.
+  Inductive Prec e t : Prop :=
+  | prec_def:
+    forall k,
+    Edge k e t ->
+    Prec e t.
 
   Variable cg: computation_graph.
 
-  Definition ContinueRefl x := ClosTransRefl (LContinue (cg_tees cg)) x.
+  Definition HB_Edge_alt e := List.Exists (Prec e) (cg_tees cg).
 
-  Definition HB := Reaches (LPrec (cg_tees cg)).
+  Definition HB_Edge := FGraph.Edge (cg_edges cg).
+
+  Definition HB := Reaches HB_Edge.
 
   Definition MHP x y : Prop := ~ HB x y /\ ~ HB y x.
+
+  Let in_edges_to_tees:
+    forall e,
+    List.In e (cg_edges cg) ->
+    exists x, List.In x (cg_tees cg) /\ Prec e x.
+  Proof.
+    unfold cg_edges.
+    intros.
+    rewrite in_flat_map in *.
+    destruct H as (x, (Hi, He)).
+    exists x; split; auto.
+    unfold to_edges in *.
+    destruct He as [?|[?|?]]; subst.
+    - destruct x.
+      destruct ntype0;
+      eauto using prec_def, edge_fork, edge_join.
+    - eauto using prec_def, edge_continue.
+    - inversion H.
+  Qed.
+
+  Let in_tees_to_edges:
+    forall x e,
+    List.In x (cg_tees cg) ->
+    Prec e x ->
+    List.In e (cg_edges cg).
+  Proof.
+    unfold cg_edges.
+    intros.
+    rewrite in_flat_map in *.
+    exists x.
+    split; auto.
+    unfold to_edges.
+    destruct H0; inversion H0; subst; auto using in_eq, in_cons.
+  Qed.
+
+  Lemma hb_edge_spec:
+    forall e,
+    HB_Edge e <-> HB_Edge_alt e.
+  Proof.
+    unfold HB_Edge, HB_Edge_alt, FGraph.Edge;
+    split; intros.
+    - rewrite Exists_exists.
+      auto.
+    - rewrite Exists_exists in *.
+      destruct H as (?, (?,?)).
+      eauto.
+  Qed.
 
   (** Comparable with respect to the happens-before relation [n1 < n2 \/ n2 < n1] *)
 
@@ -413,76 +543,97 @@ End Defs.
 
 End CG.
 
+Section HB.
+
+  Let walk2_edge_false:
+    forall {A:Type} (x y:A) w,
+    ~ Walk2 (fun _ => False) x y w.
+  Proof.
+    intuition.
+    destruct H.
+    destruct w.
+    - eauto using starts_with_inv_nil.
+    - eapply walk_to_edge; eauto using in_eq.
+  Qed.
+
+  Let reaches_edge_false:
+    forall {A:Type} (x y:A),
+    ~ Reaches (fun _ => False) x y.
+  Proof.
+    intuition.
+    inversion H.
+    apply walk2_edge_false in H0; auto.
+  Qed.
+
+  Lemma hb_make_cg_absurd:
+    forall a x y,
+    ~ HB (make_cg a) x y.
+  Proof.
+    intros.
+    compute.
+    apply reaches_edge_false.
+  Qed.
+
+End HB.
+
 Module WellFormed.
   Import Trace.
 
-  Inductive Spawns : trace -> tid -> list tid -> Prop :=
-  | spawns_nil:
+  Inductive Forks : trace -> tid -> list tid -> Prop :=
+  | forks_nil:
     forall x,
-    Spawns nil x (x::nil)
-  | spawns_cons_spawn:
+    Forks nil x (x::nil)
+  | forks_cons_fork:
     forall ts l z x y,
     (* x -> y *)
     List.In x l ->
     ~ List.In y l ->
-    Spawns ts z l ->
-    Spawns (Some {|op_t:=SPAWN; op_src:=x; op_dst:=y |}::ts) z (y::l)
-  | spawns_cons_join:
+    Forks ts z l ->
+    Forks ({|op_t:=FORK; op_src:=x; op_dst:=y |}::ts) z (y::l)
+  | forks_cons_join:
     forall ts l x y z,
     List.In x l ->
     List.In y l ->
-    Spawns ts z l ->
-    Spawns (Some {|op_t:=JOIN; op_src:=x; op_dst:=y |}::ts) z l
-  | spawns_cons_none:
-    forall ts l z,
-    Spawns ts z l ->
-    Spawns (None::ts) z l.
+    Forks ts z l ->
+    Forks ({|op_t:=JOIN; op_src:=x; op_dst:=y |}::ts) z l.
 
   Inductive Joins: trace -> list tid -> Prop :=
   | joins_nil:
     Joins nil nil
-  | joins_cons_spawn:
+  | joins_cons_fork:
     forall ts l x y,
     ~ List.In x l ->
     ~ List.In y l ->
     Joins ts l ->
-    Joins (Some {|op_t:=SPAWN; op_src:=x; op_dst:=y |}::ts) l
+    Joins ({|op_t:=FORK; op_src:=x; op_dst:=y |}::ts) l
   | joins_cons_join:
     forall ts l x y,
     ~ List.In x l ->
     Joins ts l ->
-    Joins (Some {|op_t:=JOIN; op_src:=x; op_dst:=y |}::ts) l
-  | joins_cons_none:
-    forall ts l,
-    Joins ts l ->
-    Joins (None::ts) l.
+    Joins ({|op_t:=JOIN; op_src:=x; op_dst:=y |}::ts) l.
 
   Inductive Running : trace -> tid -> list tid -> Prop :=
   | running_nil:
     forall x,
     Running nil x (x::nil)
-  | running_cons_spawn:
+  | running_cons_fork:
     forall ts l x y z,
     (* x -> y *)
     List.In x l ->
     ~ List.In y l ->
     Running ts z l ->
-    Running (Some {|op_t:=SPAWN; op_src:=x; op_dst:=y |}::ts) z (y::l)
+    Running ({|op_t:=FORK; op_src:=x; op_dst:=y |}::ts) z (y::l)
   | running_cons_join:
     forall ts l x y z,
     List.In x l ->
     Running ts z l ->
-    Running (Some {|op_t:=JOIN; op_src:=x; op_dst:=y |}::ts) z (remove TID.eq_dec y l)
-  | running_cons_none:
-    forall ts l z,
-    Running ts z l ->
-    Running (None::ts) z l.
+    Running ({|op_t:=JOIN; op_src:=x; op_dst:=y |}::ts) z (remove TID.eq_dec y l).
 
   Require Import Aniceto.List.
 
-  Lemma spawns_no_dup:
+  Lemma forks_no_dup:
     forall ts x l,
-    Spawns ts x l  ->
+    Forks ts x l  ->
     NoDup l.
   Proof.
     induction ts; intros. {
@@ -494,10 +645,10 @@ Module WellFormed.
     eauto using NoDup_cons.
   Qed.
 
-  Lemma running_incl_spawned:
+  Lemma running_incl_forked:
     forall ts ks rs x,
     Running ts x rs ->
-    Spawns ts x ks ->
+    Forks ts x ks ->
     incl rs ks.
   Proof.
     induction ts; intros. {
@@ -510,19 +661,17 @@ Module WellFormed.
     - eauto using incl_cons_cons.
     - inversion H0; subst.
       eauto using remove_incl, incl_tran.
-    - inversion H0.
-      eauto.
   Qed.
 
-  Lemma in_running_in_spawn:
+  Lemma in_running_in_fork:
     forall ts vs rs x y,
     Running ts x rs ->
-    Spawns ts x vs ->
+    Forks ts x vs ->
     List.In y rs ->
     List.In y vs.
   Proof.
     intros.
-    assert (incl rs vs) by eauto using running_incl_spawned.
+    assert (incl rs vs) by eauto using running_incl_forked.
     auto.
   Qed.
 
@@ -536,12 +685,10 @@ Module WellFormed.
       inversion H; inversion H0;
       intuition.
     }
-    destruct a as [(a,src,dst)|].
-    - destruct a; inversion H; inversion H0; subst; clear H H0.
-      + destruct H1; subst; eauto.
-      + eauto using remove_in.
-    - inversion H; inversion H0; subst; clear H H0.
-      eauto.
+    destruct a as (a,src,dst).
+    destruct a; inversion H; inversion H0; subst; clear H H0.
+    + destruct H1; subst; eauto.
+    + eauto using remove_in.
   Qed.
 
   Lemma joins_not_in_running:
@@ -554,24 +701,17 @@ Module WellFormed.
       inversion H; inversion H0; subst.
       inversion H1.
     }
-    destruct a as [(a,src,dst)|].
-    - destruct a; inversion H; inversion H0; subst; clear H H0.
-      + unfold not; intros Hx.
-        destruct Hx.
-        * subst.
-          contradiction.
-        * assert (Hx := IHts _ _ _ H9 H16 _ H1).
-          contradiction.
-      + unfold not; intros Hx.
-        apply remove_in in Hx.
-        assert (Hy := IHts _ _ _ H8 H14 _ H1).
-        contradiction.
-    - inversion H; inversion H0.
-      eauto.
+    destruct a as (a,src,dst).
+    destruct a; inversion H; inversion H0; subst; clear H H0.
+    + unfold not; intros Hx.
+      destruct Hx.
+      * subst; contradiction.
+      * assert (Hx := IHts _ _ _ H9 H16 _ H1); contradiction.
+    + unfold not; intros Hx.
+      apply remove_in in Hx.
+      assert (Hy := IHts _ _ _ H8 H14 _ H1).
+      contradiction.
   Qed.
-
-  Require Import Coq.Lists.ListSet.
-  Require Import Aniceto.ListSet.
 
   Lemma running_no_dup:
     forall ts rs x,
@@ -582,1242 +722,69 @@ Module WellFormed.
     - auto using no_dup_cons_nil.
     - eauto using NoDup_cons.
     - eauto using no_dup_remove.
-    - eauto.
+  Qed.
+
+  Let forks_in_cg:
+    forall l x t cg ts,
+    CG x l cg ->
+    Forks l x ts ->
+    List.In t ts ->
+    In t cg.
+  Proof.
+    induction l; intros. {
+      inversion H0; subst.
+      destruct H1. {
+        subst.
+        inversion H; subst.
+        auto using in_make.
+      }
+      inversion H1.
+    }
+    inversion H0; subst; clear H0.
+    - destruct H1;
+      inversion H; subst; clear H.
+      + auto using in_fork_1.
+      + eauto using in_fork_2.
+    - inversion H; subst; clear H.
+      eauto using in_join_2.
+  Qed.
+
+  (**
+   Building a CG from a trace.
+   *)
+  Lemma cg_spec:
+    forall x l ts,
+    Forks l x ts ->
+    CG x l (trace_to_cg x l).
+  Proof.
+    induction l; intros. {
+      unfold trace_to_cg.
+      simpl.
+      auto using cg_nil.
+    }
+    destruct a as (t);
+    try destruct t; simpl in *;
+    inversion H; subst.
+    - eauto using cg_cons_fork, forks_in_cg.
+    - apply cg_cons_join; eauto using forks_in_cg.
   Qed.
 
 End WellFormed.
 
-Require Import Coq.Structures.OrderedTypeEx.
-Require Import Coq.Structures.OrderedType.
-Require Import Coq.FSets.FMapAVL.
-Module M := FMapAVL.Make Nat_as_OT.
-
-Module Restriction.
-  Require Import Aniceto.Graphs.FGraph.
-  Section Defs.
-
-  Let vertex_mem (vs:list tid) (x:tid) := ListSet.set_mem TID.eq_dec x vs.
-
-  Let edge_mem vs (e:tid*tid) := let (x,y) := e in andb (vertex_mem vs x) (vertex_mem vs y).
-
-  Definition edge_eq_dec := Pair.pair_eq_dec TID.eq_dec.
-
-  Definition restriction vs es := filter (edge_mem vs) es.
-
-  Lemma restriction_incl:
-    forall vs es,
-    incl (restriction vs es) es.
-  Proof.
-    intros.
-    unfold restriction.
-    auto using List.filter_incl.
-  Qed.
-
-  Let vertex_mem_true_to_prop:
-    forall x l,
-    vertex_mem l x = true ->
-    List.In x l.
-  Proof.
-    unfold vertex_mem.
-    intros.
-    apply ListSet.set_mem_correct1 in H.
-    auto.
-  Qed.
-
-  Let vertex_mem_false_to_prop:
-    forall x l,
-    vertex_mem l x = false ->
-    ~ List.In x l.
-  Proof.
-    unfold vertex_mem.
-    intros.
-    apply ListSet.set_mem_complete1 in H.
-    auto.
-  Qed.
-
-  Let edge_mem_true_to_prop:
-    forall rs x1 x2,
-    edge_mem rs (x1, x2) = true ->
-    List.In x1 rs /\ List.In x2 rs.
-  Proof.
-    unfold edge_mem.
-    intros.
-    remember (vertex_mem _ x1) as b1.
-    remember (vertex_mem _ x2) as b2.
-    symmetry in Heqb1; symmetry in Heqb2.
-    destruct b1, b2; subst; try inversion H.
-    auto using vertex_mem_true_to_prop.
-  Qed.
-
-  Let edge_mem_false_to_prop:
-    forall rs x1 x2,
-    edge_mem rs (x1, x2) = false ->
-    ~ List.In x1 rs \/ ~ List.In x2 rs.
-  Proof.
-    unfold edge_mem.
-    intros.
-    rewrite Bool.andb_false_iff in H.
-    destruct H;
-    eauto using vertex_mem_false_to_prop.
-  Qed.
-
-  Let edge_mem_true_from_prop:
-    forall rs x1 x2,
-    List.In x1 rs ->
-    List.In x2 rs ->
-    edge_mem rs (x1, x2) = true.
-  Proof.
-    intros.
-    remember (edge_mem _ _).
-    symmetry in Heqb.
-    destruct b; auto.
-    apply edge_mem_false_to_prop in Heqb.
-    destruct Heqb; contradiction.
-  Qed.
-
-  Let restriction_inv_edge:
-    forall x1 x2 rs es,
-    List.In (x1, x2) (restriction rs es) ->
-    List.In x1 rs /\ List.In x2 rs.
-  Proof.
-    unfold restriction.
-    intros.
-    apply filter_In in H.
-    destruct H.
-    auto.
-  Qed.
-
-  Lemma restriction_in_1:
-    forall rs es x,
-    Graph.In (Edge (restriction rs es)) x ->
-    List.In x rs.
-  Proof.
-    unfold Edge.
-    intros.
-    destruct H as ((x1,x2),(He,inP)).
-    apply restriction_inv_edge in He.
-    destruct He.
-    destruct inP; simpl in *; subst; auto.
-  Qed.
-
-  Lemma restriction_in_2:
-    forall x1 x2 rs es,
-    List.In (x1, x2) es ->
-    List.In x1 rs ->
-    List.In x2 rs ->
-    List.In (x1, x2) (restriction rs es).
-  Proof.
-    unfold restriction.
-    intros.
-    apply List.filter_true_to_in; auto.
-  Qed.
-
-  End Defs.
-End Restriction.
-
-Module SafeJoins.
+Module Lang.
   Import Trace.
-  Import Restriction.
-  Require Import Aniceto.Graphs.FGraph.
 
-  Section Defs.
-  Notation known := (list (tid*tid)).
-
-  Definition safe_join_of t (e:tid*tid) := let (x,y) := e in if TID.eq_dec x t then Some y else None.
-
-  Definition get_safe_joins x := List.omap (safe_join_of x).
-
-  Definition copy_from (x y:tid) k := map (fun z => (y, z)) (get_safe_joins x k).
-
-  Definition spawn (x y:tid) (k:known) : known :=
-  copy_from x y k ++ (x,y) :: k.
-
-  Definition join (x y:tid) (k:known) : known :=
-  copy_from y x k ++ k.
-
-  Definition eval (o:option op) :=
-  match o with
-  | Some o =>
-    let f := match op_t o with
-      | SPAWN => spawn
-      | JOIN => join 
-      end
-    in
-    f (op_src o) (op_dst o)
-  | _ => fun k => k
-  end.
-
-  Inductive Check (k:known) : option op -> Prop :=
-  | check_spawn:
-    forall x y,
-    x <> y ->
-    ~ In (Edge k) y ->
-    Check k (Some {| op_t := SPAWN; op_src:= x; op_dst:= y|})
-  | check_join:
-    forall x y,
-    Edge k (x,y) ->
-    Check k (Some {| op_t := JOIN; op_src := x; op_dst:= y|})
-  | check_none:
-    Check k None.
-
-  Inductive Safe : trace -> known -> Prop :=
-  | safe_nil:
-    Safe nil nil
-  | safe_cons:
-    forall o l k,
-    Check k o ->
-    Safe l k ->
-    Safe (o::l) (eval o k).
-
-  Import Aniceto.Graphs.DAG.
-
-  Let copy_from_eq:
-    forall x y z k,
-    copy_from x y ((x,z) :: k) = (y,z) :: copy_from x y k.
-  Proof.
-    intros.
-    unfold copy_from.
-    simpl.
-    destruct (TID.eq_dec x x). {
-      auto.
-    }
-    contradiction n.
-    apply TID.eq_refl.
-  Qed.
-
-  Let copy_from_neq:
-    forall x y a b k,
-    a <> x ->
-    copy_from x y ((a,b) :: k) = copy_from x y k.
-  Proof.
-    intros.
-    unfold copy_from.
-    simpl.
-    destruct (TID.eq_dec a x). {
-      contradiction H.
-    }
-    auto.
-  Qed.
-
-  Let copy_from_spec_1:
-    forall k x y z, List.In (x,z) k -> List.In (y,z) (copy_from x y k).
-  Proof.
-    induction k as [|(a,b)]; intros. {
-      inversion H.
-    }
-    destruct (TID.eq_dec a x); rewrite tid_eq_rw in *. {
-      subst.
-      rewrite copy_from_eq.
-      destruct H. {
-        inversion H; subst.
-        auto using in_eq.
-      }
-      apply in_cons.
-      auto using in_cons.
-    }
-    rewrite copy_from_neq; auto.
-    destruct H. {
-      inversion H.
-      contradiction.
-    }
-    auto.
-  Qed.
-
-  Let copy_from_spec_2:
-    forall k x y z, List.In (y,z) (copy_from x y k) -> List.In (x,z) k.
-  Proof.
-    induction k as [|(a,b)]; intros. {
-      inversion H.
-    }
-    destruct (TID.eq_dec a x); rewrite tid_eq_rw in *. {
-      subst.
-      rewrite copy_from_eq in *.
-      destruct H. {
-        inversion H; subst.
-        auto using in_eq.
-      }
-      eauto using in_cons.
-    }
-    rewrite copy_from_neq in *; auto.
-    eauto using in_cons.
-  Qed.
-
-  Let copy_from_inv_eq:
-    forall a b x y k,
-    List.In (a, b) (copy_from x y k) ->
-    a = y.
-  Proof.
-    induction k as [|(v1,v2)]; intros. {
-      inversion H.
-    }
-    destruct (TID.eq_dec v1 x); rewrite tid_eq_rw in *. {
-      subst.
-      rewrite copy_from_eq in *.
-      destruct H. {
-        inversion H; subst.
-        trivial.
-      }
-      auto.
-    }
-    rewrite copy_from_neq in *; auto.
-  Qed.
-
-  Let reaches_edge_absurd_nil:
-    forall {A:Type} (x:A),
-    ~ Reaches (Edge nil) x x.
-  Proof.
-    intros.
-    unfold not; intros.
-    inversion H.
-    inversion H0.
-    destruct H1 as (?,(?,(?,?))).
-    subst.
-    inversion H3.
-    inversion H6.
-  Qed.
-
-  Require Import Aniceto.Pair.
-
-  Let dag_spawn_aux_0:
-    forall l k x y,
-    DAG (Edge k) ->
-    x <> y ->
-    ~ In (Edge k) y ->
-    incl l k ->
-    DAG (Edge (copy_from x y l ++ (x,y)::k)).
-  Proof.
-    induction l; intros. {
-      simpl in *.
-      apply f_dag_cons; auto using TID.eq_dec.
-      unfold not; intros X.
-      contradiction H1; eauto using reaches_to_in_fst.
-    }
-    assert (DAG (Edge (copy_from x y l ++ (x,y) ::k))) by
-          eauto using List.incl_strengthten; clear IHl.
-    destruct a as (a,b).
-    destruct (TID.eq_dec a x); rewrite tid_eq_rw in *.
-    - subst.
-      rewrite copy_from_eq. 
-      simpl.
-      assert (y <> b). {
-        unfold not; intros; subst.
-        assert (List.In (x,b) k) by (unfold incl in *; auto using in_eq).
-        assert (Edge k (x,b)) by (unfold Edge; auto).
-        contradiction H1.
-        eauto using in_right.
-      }
-      apply f_dag_cons; auto using TID.eq_dec.
-      remember (_ ++ _ :: k) as es.
-      unfold not; intros.
-      (* for b to reach y in ES, then it must pass through (x,y) *)
-      inversion H5 as (w,Hw2).
-      assert (w =  (x,y) :: nil). {
-        inversion Hw2; subst.
-        inversion H7 as ((v,?),(?,?)); simpl in *; subst.
-        rename H9 into E.
-        remember (_ ++ _) as es.
-        assert (v = x). {
-          assert (Hi := E).
-          apply end_to_edge with (Edge:=Edge es) in Hi; auto.
-          subst.
-          unfold Edge in Hi.
-          rewrite in_app_iff in Hi.
-          destruct Hi.
-          - assert (v = y) by eauto; subst.
-            apply copy_from_spec_2 in H9.
-            assert (List.In (x,y) k); (apply List.incl_strengthten in H2; auto).
-            contradiction H1.
-            assert (Edge k (x,y)) by (unfold Edge;auto).
-            eauto using in_right.
-          - destruct H9 as [X|X]. {
-              inversion X; subst; auto.
-            }
-            contradiction H1.
-            assert (Edge k (v,y)) by (unfold Edge;auto).
-            eauto using in_right.
-        }
-        subst.
-        assert (List.In (x,y) w) by auto using end_in.
-        apply end_to_append in E.
-        destruct E as (w', ?); subst.
-        destruct w'. {
-          auto.
-        }
-        apply walk2_split_app in Hw2.
-        destruct Hw2.
-        remember (_ ++ (_ :: k)) as es.
-        assert (Reaches (Edge es) b x) by eauto using reaches_def.
-        assert (Reaches (Edge es) x b). {
-          assert (Edge es (x,b)). {
-            unfold Edge, incl in *.
-            subst.
-            rewrite in_app_iff.
-            eauto using in_eq, in_cons.
-          }
-          auto using edge_to_reaches.
-        }
-        assert (n: Reaches (Edge es) b b) by eauto using reaches_trans.
-        apply H3 in n.
-        contradiction.
-      } (* w =  (x,y) :: nil *)
-      subst.
-      assert (b = x). {
-        inversion Hw2; subst.
-        apply starts_with_eq in H6.
-        auto.
-      }
-      subst.
-      remember (_ ++ (_ :: k)) as es.
-      assert (n: Reaches (Edge es) x x). {
-        assert (Edge es (x,x)). {
-          unfold Edge.
-          subst.
-          rewrite in_app_iff.
-          eauto using in_eq, in_cons.
-        }
-        auto using edge_to_reaches.
-      }
-      apply H3 in n; contradiction.
-    - rewrite copy_from_neq; auto.
-  Qed.
-
-  Let dag_spawn:
-    forall k x y,
-    DAG (Edge k) ->
-    x <> y ->
-    ~ In (Edge k) y ->
-    DAG (Edge (spawn x y k)).
-  Proof.
-    unfold spawn.
-    intros.
-    apply dag_spawn_aux_0; auto using incl_refl.
-  Qed.
-
-  Let dag_join_aux_0:
-    forall l k x y,
-    DAG (Edge k) ->
-    x <> y ->
-    Edge k (x,y) ->
-    incl l k ->
-    DAG (Edge (copy_from y x l ++ k)).
-  Proof.
-    induction l; intros. { auto. }
-    assert (DAG (Edge (copy_from y x l ++ k))) by
-          eauto using List.incl_strengthten; clear IHl.
-    destruct a as (a,b).
-    destruct (TID.eq_dec a y); rewrite tid_eq_rw in *.
-    - subst.
-      rewrite copy_from_eq. 
-      simpl.
-      assert (x <> b). {
-        unfold not; intros; subst.
-        assert (List.In (y,b) k) by (unfold incl in *; auto using in_eq).
-        assert (Edge k (y,b)) by (unfold Edge; auto).
-        assert (Reaches (Edge k) y b) by auto using edge_to_reaches.
-        assert (Reaches (Edge k) b y) by auto using edge_to_reaches.
-        assert (n: Reaches (Edge k) y y) by eauto using reaches_trans.
-        apply H in n; contradiction.
-      }
-      apply f_dag_cons_reaches; auto using TID.eq_dec.
-        remember ( _ ++ _ ) as es.
-        assert (Reaches (Edge es) y b). {
-          assert (Edge es (y,b)). {
-            unfold Edge, incl in *.
-            subst.
-            rewrite in_app_iff.
-            eauto using in_eq, in_cons.
-          }
-          auto using edge_to_reaches.
-        }
-        assert (Reaches (Edge es) x y). {
-          assert (Edge es (x,y)). {
-            unfold Edge, incl in *.
-            subst.
-            rewrite in_app_iff.
-            eauto using in_eq, in_cons.
-          }
-          auto using edge_to_reaches.
-        }
-        eauto using reaches_trans.
-    - rewrite copy_from_neq; auto.
-  Qed.
-
-  Let dag_join:
-    forall k x y,
-    DAG (Edge k) ->
-    Edge k (x,y) ->
-    DAG (Edge (join x y k)).
-  Proof.
-    intros.
-    unfold join.
-    assert (x <> y). {
-      unfold not; intros; subst.
-      assert (n: Reaches (Edge k) y y) by auto using edge_to_reaches.
-      apply H in n.
-      contradiction.
-    }
-    apply dag_join_aux_0; auto using incl_refl.
-  Qed.
-
-  Lemma eval_preserves_dag:
-    forall k o,
-    Check k o ->
-    DAG (Edge k) ->
-    DAG (Edge (eval o k)).
-  Proof.
-    intros.
-    destruct o; auto.
-    inversion H; subst; simpl; auto.
-  Qed.
-
-  (**
-    If the safe-joins graph that yields a trace is well-formed, then
-    the safe-joins graph is a DAG.
-    *)
-
-  Theorem safe_to_dag:
-    forall t k,
-    Safe t k ->
-    DAG (Edge k).
-  Proof.
-    intros.
-    induction H. {
-      auto using f_dag_nil.
-    }
-    auto using eval_preserves_dag.
-  Qed.
-
-  Notation R_Edge rs k := (Edge (restriction rs k)).
-
-  Notation R_DAG rs k := (DAG (R_Edge rs k)).
-
-  Import WellFormed.
-
-  Let running_infimum:
-    forall rs k,
-    restriction rs k <> nil ->
-    R_DAG rs k ->
-    exists x, Graph.In (R_Edge rs k) x /\
-      forall y, ~ Reaches (R_Edge rs k) x y.
-  Proof.
-    intros.
-    apply dag_infimum; auto using TID.eq_dec.
-  Qed.
-
-
-  Let safe_to_r_dag:
-    forall t k rs,
-    Safe t k ->
-    R_DAG rs k.
-  Proof.
-    intros.
-    apply safe_to_dag in H.
-    apply f_dag_incl with (es:=k); auto using restriction_incl.
-  Qed.
-
-  Let progress_0:
-    forall t k rs,
-    Safe t k ->
-    (restriction rs k) <> nil ->
-    exists x, List.In x rs /\ forall y, Edge k (x,y) -> ~ List.In y rs.
-  Proof.
-    intros.
-    assert (Hx:
-      exists x, Graph.In (R_Edge rs k) x /\
-      forall y, ~ Reaches (R_Edge rs k) x y). {
-        eapply running_infimum; eauto.
-    }
-    destruct Hx as (x, (Hin, Hy)).
-    exists x.
-    split; eauto using restriction_in_1.
-    unfold not;
-    intros y He Hx.
-    assert (Hz := Hy y); clear Hy.
-    contradiction Hz; clear Hz.
-    assert (List.In x rs). {
-      eauto using restriction_in_1.
-    }
-    assert (R_Edge rs k (x,y)). {
-      unfold Edge.
-      auto using restriction_in_2.
-    }
-    auto using edge_to_reaches.
-  Qed.
-
-  Theorem progress:
-    forall t k rs,
-    Safe t k ->
-    rs <> nil ->
-    exists x, List.In x rs /\ forall y, Edge k (x,y) -> ~ List.In y rs.
-  Proof.
-    intros.
-    remember (restriction rs k) as l.
-    destruct l. {
-      subst.
-      destruct rs. { contradiction H0; auto. }
-      exists t0.
-      assert (List.In t0 (t0::rs)) by auto using in_eq.
-      split. { auto. }
-      intros.
-      unfold not; intros.
-      assert (List.In (t0, y) (restriction (t0::rs) k)) by auto using restriction_in_2.
-      rewrite <- Heql in *.
-      inversion H4.
-    }
-    assert (restriction rs k <> nil). {
-      intuition.
-      rewrite H1 in *.
-      inversion Heql.
-    }
-    eauto.
-  Qed.
-
-  End Defs.
-
-  Module Lang.
-    Fixpoint from_trace ts := 
-    match ts with
-    | nil => nil
-    | o :: ts => eval o (from_trace ts)
-    end.
-
-    Definition effects_to_sj ts := from_trace (from_effects ts).
-
-    Definition Safe ts := Safe (Trace.from_effects ts) (effects_to_sj ts).
-  End Lang.
-End SafeJoins.
-
-
-Module Known.
-  Import Trace.
-  Import Restriction.
-  Require Import Aniceto.Graphs.FGraph.
-
-  Section Defs.
-  Definition known := MT.t (list tid).
-  Definition make (x:tid) : known := (MT.add x nil (@MT.empty (list tid))).
-
-  Definition spawn (x y:tid) (k:known) : known :=
-  match MT.find x k with
-  | Some l => (MT.add x (y::l)) (MT.add y l k)
-  | _ => k
-  end.
-
-  Definition join (x y:tid) (k:known) : known :=
-  match (MT.find x k, MT.find y k) with
-  | (Some lx,Some ly) =>
-    MT.add x (ly ++ lx) k
-  | _ => k
-  end.
-
-  Definition eval (o:option op) :=
-  match o with
-  | Some o =>
-    let f := match op_t o with
-      | SPAWN => spawn
-      | JOIN => join 
-      end
-    in
-    f (op_src o) (op_dst o)
-  | _ => fun k => k
-  end.
-
-  Inductive Check (k:known) : option op -> Prop :=
-  | check_spawn:
-    forall x y,
-    MT.In x k ->
-    ~ MT.In y k ->
-    Check k (Some {| op_t := SPAWN; op_src:= x; op_dst:= y|})
-  | check_join:
-    forall x y lx ly,
-    MT.MapsTo x lx k ->
-    MT.MapsTo y ly k ->
-    List.In y lx ->
-    ~ List.In x ly ->
-    Check k (Some {| op_t := JOIN; op_src := x; op_dst:= y|})
-  | check_none:
-    Check k None.
-
-  Fixpoint from_trace x ts :=
-  match ts with
-  | nil => make x
-  | o :: ts => eval o (from_trace x ts)
-  end.
-
-  Inductive Safe : trace -> tid -> known -> Prop :=
-  | safe_nil:
-    forall x,
-    Safe nil x (make x)
-  | safe_cons:
-    forall o l z k,
-    Check k o ->
-    Safe l z k ->
-    Safe (o::l) z (eval o k).
-
-  Inductive SpawnEdges : trace -> list (tid*tid) -> Prop :=
-  | spawn_edges_nil:
-    SpawnEdges nil nil
-  | spawn_edges_cons_spawn:
-    forall x y l e,
-    SpawnEdges l e ->
-    SpawnEdges (Some {| op_t:=SPAWN; op_src:=x; op_dst:=y|}::l) ((x,y)::e)
-  | spawn_edges_cons_join:
-    forall l e x y,
-    SpawnEdges l e ->
-    SpawnEdges (Some {| op_t:=JOIN; op_src:=x; op_dst:=y|}::l) e
-  | spawn_edges_cons_none:
-    forall l e,
-    SpawnEdges l e ->
-    SpawnEdges (None::l) e.  
-
-  Definition to_spawn_edge e :=
+  Definition from_effect (e:Lang.effect) :=
   match e with
-  | Some {| op_t:=SPAWN; op_src:=x; op_dst:=y|} => Some (x,y)
+  | (x, Lang.FUTURE y) => Some {|op_t:=FORK; op_src:=x; op_dst:=y|}
+  | (x, Lang.FORCE y) => Some {|op_t:=JOIN; op_src:=x; op_dst:=y|}
   | _ => None
   end.
 
-  Definition spawn_edges (ts:trace) := List.omap to_spawn_edge ts.
+  Definition from_effects := List.omap from_effect.
 
-  Inductive WellFormed (k:known) :=
-  | well_formed_def:
-    (forall t l, MT.MapsTo t l k -> ~ List.In t l) ->
-    (forall x y l, MT.MapsTo x l k -> List.In y l -> MT.In y k) ->
-    WellFormed k.
+  (** Compute a CG from a trace of our language. *)
 
-  Require Import Bijection.
-  Import WellFormed.
+  Definition effects_to_cg (x:tid) ts := trace_to_cg x (from_effects ts).
 
-  (** The spawn-tree is a DAG *)
-
-  Let edge_in_absurd_nil:
-    forall {A:Type} (x:A),
-    ~ Graph.In (Edge nil) x.
-  Proof.
-    intuition.
-    destruct H as (?,(n,?)).
-    destruct n.
-  Qed.
-
-  Let spawn_edges_to_spawns:
-    forall x t a vs es,
-    Spawns t a vs ->
-    SpawnEdges t es ->
-    Graph.In (Edge es) x ->
-    List.In x vs.
-  Proof.
-    induction t; intros. {
-      inversion H0; subst.
-      apply edge_in_absurd_nil in H1.
-      inversion H1.
-    }
-    inversion H; subst; clear H; inversion H0; subst; clear H0; eauto.
-    destruct H1 as (e',(He,Hi)).
-    destruct He; subst.
-    + destruct Hi as [Hi|Hi]; symmetry in Hi; simpl in *; subst; intuition.
-    + assert (Graph.In (Edge e) x) by eauto using in_def.
-      eauto using in_cons.
-  Qed.
-
-  Let make_mapsto:
-    forall x,
-    MT.MapsTo x nil (make x).
-  Proof.
-    intros.
-    unfold make.
-    auto using MT.add_1.
-  Qed.
-
-  Let make_inv_maps_to:
-    forall x y l,
-    MT.MapsTo x l (make y) ->
-    x = y /\ l = nil.
-  Proof.
-    intros.
-    unfold make in *.
-    apply MT_Facts.add_mapsto_iff in H.
-    destruct H as [(?,?)|(?,?)]; auto.
-    apply MT_Facts.empty_mapsto_iff in H0.
-    contradiction.
-  Qed.
-
-  Let spawn_inv_maps_to:
-    forall x y z l k,
-    MT.MapsTo z l (spawn x y k) ->
-    MT.MapsTo z l k \/
-    (z = x /\ exists l', l = y :: l' /\ MT.MapsTo x l' k) \/
-    (x <> z /\ y = z /\ MT.MapsTo x l k).
-  Proof.
-    intros.
-    unfold spawn in *.
-    destruct (MT_Extra.find_rw x k) as [(He,n)|(?,(He,?))]; rewrite He in *.
-    - auto.
-    - apply MT_Facts.add_mapsto_iff in H.
-      destruct H as [(?,?)|(?,?)].
-      + right; left.
-        intuition.
-        exists x0.
-        intuition.
-      + apply MT_Facts.add_mapsto_iff in H1.
-        destruct H1 as [(?,?)|(?,?)].
-        * right; right.
-          subst; auto.
-        * intuition.
-  Qed.
-
-  Let join_inv_maps_to:
-    forall x y z l k,
-    MT.MapsTo z l (join x y k) ->
-    MT.MapsTo z l k \/
-    (exists lx ly, MT.MapsTo x lx k /\ MT.MapsTo y ly k /\ l = ly ++ lx /\ z = x).
-  Proof.
-    unfold join.
-    intros.
-    destruct (MT_Extra.find_rw x k) as [(He,n)|(?,(He,?))]; rewrite He in *. {
-      intuition.
-    }
-    destruct (MT_Extra.find_rw y k) as [(He',n)|(?,(He',?))]; rewrite He' in *. {
-      intuition.
-    }
-    clear He He'.
-    apply MT_Facts.add_mapsto_iff in H.
-    destruct H as [(?,?)|(?,?)].
-    - subst.
-      right.
-      exists x0.
-      eauto.
-    - intuition.
-  Qed.
-
-  Let spawn_mapsto_neq:
-    forall (x y:tid) l (k:known),
-    y <> x ->
-    MT.MapsTo x l k ->
-    MT.MapsTo y l (spawn x y k).
-  Proof.
-    intros.
-    unfold spawn.
-    destruct (MT_Extra.find_rw x k) as [(He,n)|(?,(He,?))]; rewrite He.
-    - contradiction n; eauto using MT_Extra.mapsto_to_in.
-    - assert (x0 = l) by eauto using MT_Facts.MapsTo_fun; subst.
-      eauto using MT.add_2, MT.add_1.
-  Qed.
-
-  Let spawn_mapsto_inv_1:
-    forall x y l k,
-    MT.In x k ->
-    MT.MapsTo x l (spawn x y k) ->
-    exists l', (l = y::l' /\ MT.MapsTo x l' k).
-  Proof.
-    unfold spawn.
-    intros.
-    destruct (MT_Extra.find_rw x k) as [(He,n)|(?,(He,?))]; rewrite He in *.
-    - contradiction.
-    - apply MT_Facts.add_mapsto_iff in H0.
-      destruct H0 as [(?,?)|(?,?)].
-      + subst.
-        eauto.
-      + contradiction H0; auto.
-  Qed.
-
-  Let spawn_mapsto_eq:
-    forall x y k l,
-    MT.MapsTo x l k ->
-    MT.MapsTo x (y::l) (spawn x y k).
-  Proof.
-    intros.
-    unfold spawn.
-    destruct (MT_Extra.find_rw x k) as [(He,n)|(?,(He,?))]; rewrite He.
-    - contradiction n; eauto using MT_Extra.mapsto_to_in.
-    - assert (x0 = l) by eauto using MT_Facts.MapsTo_fun; subst.
-      eauto using MT.add_1.
-  Qed.
-
-  Let spawn_mapsto_eq_spawned:
-    forall x y k l,
-    MT.MapsTo x l k ->
-    x <> y ->
-    MT.MapsTo y l (spawn x y k).
-  Proof.
-    intros.
-    unfold spawn.
-    destruct (MT_Extra.find_rw x k) as [(He,n)|(?,(He,?))]; rewrite He.
-    - contradiction n; eauto using MT_Extra.mapsto_to_in.
-    - assert (x0 = l) by eauto using MT_Facts.MapsTo_fun; subst.
-      eauto using MT.add_2, MT.add_1.
-  Qed.
-
-  Let spawn_mapsto_eq_spawner:
-    forall x y k l,
-    MT.In x k ->
-    x <> y ->
-    MT.MapsTo y l (spawn x y k) ->
-    MT.MapsTo x l k.
-  Proof.
-    intros.
-    unfold spawn in *.
-    destruct (MT_Extra.find_rw x k) as [(He,n)|(?,(He,?))]; rewrite He in *.
-    - contradiction n; eauto using MT_Extra.mapsto_to_in.
-    - clear He H.
-      apply MT_Facts.add_mapsto_iff in H1.
-      destruct H1 as [(?,?)|(?,?)].
-      + contradiction.
-      + apply MT_Facts.add_mapsto_iff in H1.
-        destruct H1 as [(?,?)|(?,?)]; subst; auto.
-        contradiction H1; trivial.
-  Qed.
-
-  Let spawn_mapsto_neq_neq:
-    forall x y z l k,
-    z <> x ->
-    z <> y ->
-    MT.MapsTo z l k ->
-    MT.MapsTo z l (spawn x y k).
-  Proof.
-    intros.
-    unfold spawn.
-    destruct (MT_Extra.find_rw x k) as [(He,n)|(?,(He,?))]; rewrite He.
-    - auto.
-    - eauto using MT.add_2.
-  Qed.
-
-  Let spawn_mapsto_inv_neq_neq:
-    forall x y z l k,
-    z <> x ->
-    z <> y ->
-    MT.MapsTo z l (spawn x y k) ->
-    MT.MapsTo z l k.
-  Proof.
-    unfold spawn.
-    intros.
-    destruct (MT_Extra.find_rw x k) as [(He,n)|(?,(He,?))]; rewrite He in *.
-    - auto.
-    - repeat (apply MT.add_3 in H1; auto).
-  Qed.
-
-  Let spawn_in:
-    forall x y z k,
-    MT.In z k ->
-    MT.In z (spawn x y k).
-  Proof.
-    intros.
-    unfold spawn.
-    destruct (MT_Extra.find_rw x k) as [(He,n)|(?,(He,?))];
-    rewrite He;
-    auto using MT_Extra.add_in.
-  Qed.
-
-  Let spawn_in_spawned:
-    forall x y k,
-    MT.In x k ->
-    MT.In y (spawn x y k).
-  Proof.
-    intros.
-    unfold spawn.
-    destruct (MT_Extra.find_rw x k) as [(He,n)|(?,(He,?))];
-    rewrite He.
-    - contradiction.
-    - apply MT_Extra.add_in.
-      rewrite MT_Facts.add_in_iff.
-      auto.
-  Qed.
-
-  Let join_in:
-    forall x y z k,
-    MT.In z k ->
-    MT.In z (join x y k).
-  Proof.
-    intros.
-    unfold join.
-    destruct (MT_Extra.find_rw x k) as [(He,n)|(?,(He,?))];
-    rewrite He.
-    - auto.
-    - clear He.
-      destruct (MT_Extra.find_rw y k) as [(He,n)|(?,(He,?))];
-      rewrite He;
-    auto using MT_Extra.add_in.
-  Qed.
-
-  Let edge_cons:
-    forall {A:Type} es (e e':A*A),
-    Edge es e ->
-    Edge (e' :: es) e.
-  Proof.
-    unfold Edge.
-    auto using in_cons.
-  Qed.
-
-  Let reaches_cons:
-    forall {A:Type} (x y:A) e es,
-    Reaches (Edge es) x y ->
-    Reaches (Edge (e :: es)) x y.
-  Proof.
-    eauto using reaches_impl.
-  Qed.
-
-  Lemma safe_spec:
-    forall ts x k,
-    Safe ts x k ->
-    k = from_trace x ts.
-  Proof.
-    induction ts; intros. {
-      inversion H; simpl; auto.
-    }
-    inversion H; subst.
-    simpl.
-    assert (RW: k0 = from_trace x ts) by auto.
-    rewrite RW.
-    auto.
-  Qed.
-
-  Lemma safe_fun:
-    forall ts x k1 k2,
-    Safe ts x k1 ->
-    Safe ts x k2 ->
-    k1 = k2.
-  Proof.
-    intros.
-    assert (R1 :  k1 = from_trace x ts) by auto using safe_spec.
-    assert (R2 :  k2 = from_trace x ts) by auto using safe_spec.
-    rewrite R1.
-    rewrite R2.
-    trivial.
-  Qed.
-
-  Lemma spawn_rw:
-    forall x y l k,
-    MT.MapsTo x l k ->
-    ~ MT.In (elt:=list tid) y k ->
-    spawn x y k = MT.add x (y :: l) (MT.add y l k).
-  Proof.
-    intros.
-    unfold spawn.
-    destruct (MT_Extra.find_rw x k) as [(?,?)|(l',(R,?))]. {
-      contradiction H2; eauto using MT_Extra.mapsto_to_in.
-    }
-    rewrite R.
-    assert (l' = l) by eauto using MT_Facts.MapsTo_fun; subst; auto.
-  Qed.
-
-  (** This is not true: it breaks in a spawn
-
-  Let known_to_spawn_edge:
-    forall t a es k l x y,
-    SpawnEdges t es ->
-    Safe t a k ->
-    MT.MapsTo x l k ->
-    List.In y l ->
-    WellFormed k ->
-    Reaches (Edge es) x y.
-  Proof.
-    induction t; intros. {
-      inversion H0; subst.
-      assert (X: x = a /\ l = nil) by eauto.
-      destruct X; subst.
-      inversion H2.
-    }
-    inversion H; subst; clear H.
-    - inversion H0; subst; simpl in *; clear H0.
-      inversion H10; subst; clear H10.
-      simpl in *.
-      (* --- *)
-      assert (X:=H1).
-      apply spawn_inv_maps_to in X.
-      destruct X as [?|[(?,(?,(?,?)))|(?,(?,?))]]; repeat subst.
-      + eauto.
-      + destruct H2. {
-          subst.
-          apply edge_to_reaches.
-          unfold  Edge; auto using in_eq.
-        }
-        apply spawn_mapsto_inv_1 in H1; auto.
-        destruct H1 as (?,(He,?)).
-        inversion He; clear He H6; subst.
-        rename x into l.
-        apply reaches_cons.
-        eauto.
-      + clear H4.
-  Qed.
-  *)
-
-  (* The next thing we have to do is to define a relation R, such that
-     if MT.MapsTo x l k /\ List.In y l -> x R y
-     and then prove that this yields a <
-   *)
-
-
-  Lemma in_spawns_in_known:
-    forall t x a vs k,
-    Spawns t a vs ->
-    Safe t a k ->
-    List.In x vs ->
-    MT.In x k.
-  Proof.
-    induction t; intros. {
-      inversion H; subst.
-      inversion H1.
-      - subst.
-        inversion H0; subst.
-        eauto using make_mapsto, MT_Extra.mapsto_to_in.
-      - inversion H2.
-    }
-    inversion H; subst; clear H; inversion H0; subst; clear H0; simpl; eauto.
-    destruct H1.
-    + subst.
-      simpl.
-      assert (x0 <> x). {
-        intuition; subst.
-        contradiction.
-      }
-      inversion H3; subst.
-      apply MT_Extra.in_to_mapsto in H2.
-      destruct H2 as (l', Hmt).
-      assert (MT.MapsTo x l' (spawn x0 x k0)) by eauto using spawn_mapsto_neq.
-      eauto using MT_Extra.mapsto_to_in.
-    + simpl; eauto.
-  Qed.
-
-  Let make_is_well_formed:
-    forall x,
-    WellFormed (make x).
-  Proof.
-    intros.
-    apply well_formed_def.
-    - intros.
-      apply make_inv_maps_to in H; destruct H; subst.
-      auto.
-    - intros.
-      apply make_inv_maps_to in H; destruct H; subst.
-      inversion H0.
-  Qed.
-
-  Let well_formed_not_refl:
-    forall x l k,
-    WellFormed k ->
-    MT.MapsTo x l k ->
-    ~ List.In x l.
-  Proof.
-    intros; inversion H; eauto.
-  Qed.
-
-  Lemma well_formed_range_in_dom:
-    forall x y l k,
-    WellFormed k ->
-    MT.MapsTo x l k ->
-    List.In y l ->
-    MT.In y k.
-  Proof.
-    intros; inversion H; eauto.
-  Qed.
-
-  Let spawn_is_well_formed:
-    forall x y k,
-    WellFormed k ->
-    ~ MT.In y k ->
-    WellFormed (spawn x y k).
-  Proof.
-    intros.
-    apply well_formed_def; intros. {
-    intros.
-    apply spawn_inv_maps_to in H1.
-    destruct H1 as [?|[(?,(?,(?,?)))|(?,(?,?))]]; subst; auto.
-    - eauto.
-    - unfold not; intros.
-      destruct H1.
-      + subst.
-        contradiction H0.
-        eauto using MT_Extra.mapsto_to_in.
-      + assert (~ List.In x x0) by eauto.
-        contradiction.
-    - unfold not; intros.
-      contradiction H0.
-      eauto using well_formed_range_in_dom.
-    }
-    apply spawn_inv_maps_to in H1.
-    destruct H1 as [?|[(?,(?,(?,?)))|(?,(?,?))]]; subst; eauto using well_formed_range_in_dom.
-    destruct H2; subst; eauto using MT_Extra.mapsto_to_in, well_formed_range_in_dom.
-  Qed.
-(*
-  Let well_formed_inv_spawn:
-    forall x y k,
-    ~ MT.In y k ->
-    WellFormed (spawn x y k) ->
-    WellFormed k.
-  Proof.
-    intros.
-    inversion H0.
-    apply well_formed_def; intros.
-    - destruct (TID.eq_dec t x), (TID.eq_dec t y); rewrite tid_eq_rw in *; auto; repeat subst.
-      + apply spawn_mapsto_eq with (y:=y) in H3.
-        apply well_formed_not_refl in H3; auto.
-        contradiction H3; auto using in_eq.
-      + apply spawn_mapsto_eq with (y:=y) in H3.
-        apply well_formed_not_refl in H3; auto.
-        unfold not; intros.
-        contradiction H3; auto using in_cons.
-      + assert (N: ~ MT.In y k) by eauto.
-        contradiction N; eauto using MT_Extra.mapsto_to_in.
-    - destruct (TID.eq_dec y0 x0); rewrite tid_eq_rw in *; auto; repeat subst.
-      + eauto using MT_Extra.mapsto_to_in.
-      + assert 
-        assert (MT.In y (spawn x y k)). {
-          apply H2 with (x:=x0) (l:=l).
-        }
-
-  Qed.
-*)
-  Let join_is_well_formed:
-    forall x y l k,
-    WellFormed k ->
-    MT.MapsTo y l k ->
-    ~ List.In x l ->
-    WellFormed (join x y k).
-  Proof.
-    intros.
-    apply well_formed_def.
-    - intros.
-      apply join_inv_maps_to in H2.
-      destruct H2 as [?|(?,(?,(?,(?,(?,?)))))].
-      + eauto.
-      + subst.
-        assert (x1 = l) by eauto using MT_Facts.MapsTo_fun; subst.
-        unfold not; intros.
-        apply in_app_iff in H4.
-        destruct H4.
-        * contradiction.
-        * assert (~ List.In x x0) by eauto.
-          contradiction.
-    - intros.
-      apply join_inv_maps_to in H2.
-      destruct H2 as [?|(?,(?,(?,(?,(?,?)))))].
-      + eauto using well_formed_range_in_dom.
-      + subst.
-        apply in_app_iff in H3; destruct H3; eauto using well_formed_range_in_dom.
-  Qed.
-
-  Lemma safe_to_well_formed:
-    forall t x k,
-    Safe t x k ->
-    WellFormed k.
-  Proof.
-    induction t; intros. {
-      inversion H; subst; auto.
-    }
-    inversion H; subst; clear H.
-    destruct a;
-    simpl;
-    inversion H2; eauto.
-  Qed.
-
-  (* This does not hold: 
-  Let known_to_spawn_edge:
-    forall t a es k l x y,
-    SpawnEdges t es ->
-    Safe t a k ->
-    MT.MapsTo x l k ->
-    List.In y l ->
-    Edge es (x, y).
-  *)
-
-End Defs.
-End Known.
-
+End Lang.
