src/SafeJoins.v
@@ -1,0 +1,547 @@
+Require Import Coq.Lists.List.
+
+Require Import Aniceto.List.
+Require Import Aniceto.Graphs.Graph.
+Require Import Aniceto.Graphs.FGraph.
+
+Require Import CG.
+Require Import Tid.
+
+Import Trace.
+Require Import Aniceto.Graphs.FGraph.
+
+Section Defs.
+  Notation known := (list (tid*tid)).
+
+  Definition safe_join_of t (e:tid*tid) := let (x,y) := e in if TID.eq_dec x t then Some y else None.
+
+  Definition get_safe_joins x := List.omap (safe_join_of x).
+
+  Definition copy_from (x y:tid) k := map (fun z => (y, z)) (get_safe_joins x k).
+
+  Definition fork (x y:tid) (k:known) : known :=
+  copy_from x y k ++ (x,y) :: k.
+
+  Definition join (x y:tid) (k:known) : known :=
+  copy_from y x k ++ k.
+
+  Definition eval (o:op) :=
+  let f := match op_t o with
+  | FORK => fork
+  | JOIN => join 
+  end
+  in
+  f (op_src o) (op_dst o).
+
+  Inductive Check (k:known) : op -> Prop :=
+  | check_fork:
+    forall (x y:tid),
+    x <> y ->
+    ~ Graph.In (Edge k) y ->
+    Check k {| op_t := FORK; op_src:= x; op_dst:= y|}
+  | check_join:
+    forall x y,
+    Edge k (x,y) ->
+    Check k {| op_t := JOIN; op_src := x; op_dst:= y|}.
+
+  Inductive Safe : trace -> known -> Prop :=
+  | safe_nil:
+    Safe nil nil
+  | safe_cons:
+    forall o l k,
+    Check k o ->
+    Safe l k ->
+    Safe (o::l) (eval o k).
+
+  Import Aniceto.Graphs.DAG.
+
+  Let copy_from_eq:
+    forall x y z k,
+    copy_from x y ((x,z) :: k) = (y,z) :: copy_from x y k.
+  Proof.
+    intros.
+    unfold copy_from.
+    simpl.
+    destruct (TID.eq_dec x x). {
+      auto.
+    }
+    contradiction n.
+    apply TID.eq_refl.
+  Qed.
+
+  Let copy_from_neq:
+    forall x y a b k,
+    a <> x ->
+    copy_from x y ((a,b) :: k) = copy_from x y k.
+  Proof.
+    intros.
+    unfold copy_from.
+    simpl.
+    destruct (TID.eq_dec a x). {
+      contradiction H.
+    }
+    auto.
+  Qed.
+
+  Let copy_from_spec_1:
+    forall k x y z, List.In (x,z) k -> List.In (y,z) (copy_from x y k).
+  Proof.
+    induction k as [|(a,b)]; intros. {
+      inversion H.
+    }
+    destruct (TID.eq_dec a x); rewrite tid_eq_rw in *. {
+      subst.
+      rewrite copy_from_eq.
+      destruct H. {
+        inversion H; subst.
+        auto using in_eq.
+      }
+      apply in_cons.
+      auto using in_cons.
+    }
+    rewrite copy_from_neq; auto.
+    destruct H. {
+      inversion H.
+      contradiction.
+    }
+    auto.
+  Qed.
+
+  Let copy_from_spec_2:
+    forall k x y z, List.In (y,z) (copy_from x y k) -> List.In (x,z) k.
+  Proof.
+    induction k as [|(a,b)]; intros. {
+      inversion H.
+    }
+    destruct (TID.eq_dec a x); rewrite tid_eq_rw in *. {
+      subst.
+      rewrite copy_from_eq in *.
+      destruct H. {
+        inversion H; subst.
+        auto using in_eq.
+      }
+      eauto using in_cons.
+    }
+    rewrite copy_from_neq in *; auto.
+    eauto using in_cons.
+  Qed.
+
+  Let copy_from_inv_eq:
+    forall a b x y k,
+    List.In (a, b) (copy_from x y k) ->
+    a = y.
+  Proof.
+    induction k as [|(v1,v2)]; intros. {
+      inversion H.
+    }
+    destruct (TID.eq_dec v1 x); rewrite tid_eq_rw in *. {
+      subst.
+      rewrite copy_from_eq in *.
+      destruct H. {
+        inversion H; subst.
+        trivial.
+      }
+      auto.
+    }
+    rewrite copy_from_neq in *; auto.
+  Qed.
+
+  Let reaches_edge_absurd_nil:
+    forall {A:Type} (x:A),
+    ~ Reaches (Edge nil) x x.
+  Proof.
+    intros.
+    unfold not; intros.
+    inversion H.
+    inversion H0.
+    destruct H1 as (?,(?,(?,?))).
+    subst.
+    inversion H3.
+    inversion H6.
+  Qed.
+
+  Require Import Aniceto.Pair.
+
+  Let dag_fork_aux_0:
+    forall l k x y,
+    DAG (Edge k) ->
+    x <> y ->
+    ~ Graph.In (Edge k) y ->
+    incl l k ->
+    DAG (Edge (copy_from x y l ++ (x,y)::k)).
+  Proof.
+    induction l; intros. {
+      simpl in *.
+      apply f_dag_cons; auto using TID.eq_dec.
+      unfold not; intros X.
+      contradiction H1; eauto using reaches_to_in_fst.
+    }
+    assert (DAG (Edge (copy_from x y l ++ (x,y) ::k))) by
+          eauto using List.incl_strengthten; clear IHl.
+    destruct a as (a,b).
+    destruct (TID.eq_dec a x); rewrite tid_eq_rw in *.
+    - subst.
+      rewrite copy_from_eq. 
+      simpl.
+      assert (y <> b). {
+        unfold not; intros; subst.
+        assert (List.In (x,b) k) by (unfold incl in *; auto using in_eq).
+        assert (Edge k (x,b)) by (unfold Edge; auto).
+        contradiction H1.
+        eauto using in_right.
+      }
+      apply f_dag_cons; auto using TID.eq_dec.
+      remember (_ ++ _ :: k) as es.
+      unfold not; intros.
+      (* for b to reach y in ES, then it must pass through (x,y) *)
+      inversion H5 as (w,Hw2).
+      assert (w =  (x,y) :: nil). {
+        inversion Hw2; subst.
+        inversion H7 as ((v,?),(?,?)); simpl in *; subst.
+        rename H9 into E.
+        remember (_ ++ _) as es.
+        assert (v = x). {
+          assert (Hi := E).
+          apply end_to_edge with (Edge:=Edge es) in Hi; auto.
+          subst.
+          unfold Edge in Hi.
+          rewrite in_app_iff in Hi.
+          destruct Hi.
+          - assert (v = y) by eauto; subst.
+            apply copy_from_spec_2 in H9.
+            assert (List.In (x,y) k); (apply List.incl_strengthten in H2; auto).
+            contradiction H1.
+            assert (Edge k (x,y)) by (unfold Edge;auto).
+            eauto using in_right.
+          - destruct H9 as [X|X]. {
+              inversion X; subst; auto.
+            }
+            contradiction H1.
+            assert (Edge k (v,y)) by (unfold Edge;auto).
+            eauto using in_right.
+        }
+        subst.
+        assert (List.In (x,y) w) by auto using end_in.
+        apply end_to_append in E.
+        destruct E as (w', ?); subst.
+        destruct w'. {
+          auto.
+        }
+        apply walk2_split_app in Hw2.
+        destruct Hw2.
+        remember (_ ++ (_ :: k)) as es.
+        assert (Reaches (Edge es) b x) by eauto using reaches_def.
+        assert (Reaches (Edge es) x b). {
+          assert (Edge es (x,b)). {
+            unfold Edge, incl in *.
+            subst.
+            rewrite in_app_iff.
+            eauto using in_eq, in_cons.
+          }
+          auto using edge_to_reaches.
+        }
+        assert (n: Reaches (Edge es) b b) by eauto using reaches_trans.
+        apply H3 in n.
+        contradiction.
+      } (* w =  (x,y) :: nil *)
+      subst.
+      assert (b = x). {
+        inversion Hw2; subst.
+        apply starts_with_eq in H6.
+        auto.
+      }
+      subst.
+      remember (_ ++ (_ :: k)) as es.
+      assert (n: Reaches (Edge es) x x). {
+        assert (Edge es (x,x)). {
+          unfold Edge.
+          subst.
+          rewrite in_app_iff.
+          eauto using in_eq, in_cons.
+        }
+        auto using edge_to_reaches.
+      }
+      apply H3 in n; contradiction.
+    - rewrite copy_from_neq; auto.
+  Qed.
+
+  Let dag_fork:
+    forall k x y,
+    DAG (Edge k) ->
+    x <> y ->
+    ~ Graph.In (Edge k) y ->
+    DAG (Edge (fork x y k)).
+  Proof.
+    unfold fork.
+    intros.
+    apply dag_fork_aux_0; auto using incl_refl.
+  Qed.
+
+  Let dag_join_aux_0:
+    forall l k x y,
+    DAG (Edge k) ->
+    x <> y ->
+    Edge k (x,y) ->
+    incl l k ->
+    DAG (Edge (copy_from y x l ++ k)).
+  Proof.
+    induction l; intros. { auto. }
+    assert (DAG (Edge (copy_from y x l ++ k))) by
+          eauto using List.incl_strengthten; clear IHl.
+    destruct a as (a,b).
+    destruct (TID.eq_dec a y); rewrite tid_eq_rw in *.
+    - subst.
+      rewrite copy_from_eq. 
+      simpl.
+      assert (x <> b). {
+        unfold not; intros; subst.
+        assert (List.In (y,b) k) by (unfold incl in *; auto using in_eq).
+        assert (Edge k (y,b)) by (unfold Edge; auto).
+        assert (Reaches (Edge k) y b) by auto using edge_to_reaches.
+        assert (Reaches (Edge k) b y) by auto using edge_to_reaches.
+        assert (n: Reaches (Edge k) y y) by eauto using reaches_trans.
+        apply H in n; contradiction.
+      }
+      apply f_dag_cons_reaches; auto using TID.eq_dec.
+        remember ( _ ++ _ ) as es.
+        assert (Reaches (Edge es) y b). {
+          assert (Edge es (y,b)). {
+            unfold Edge, incl in *.
+            subst.
+            rewrite in_app_iff.
+            eauto using in_eq, in_cons.
+          }
+          auto using edge_to_reaches.
+        }
+        assert (Reaches (Edge es) x y). {
+          assert (Edge es (x,y)). {
+            unfold Edge, incl in *.
+            subst.
+            rewrite in_app_iff.
+            eauto using in_eq, in_cons.
+          }
+          auto using edge_to_reaches.
+        }
+        eauto using reaches_trans.
+    - rewrite copy_from_neq; auto.
+  Qed.
+
+  Let dag_join:
+    forall k x y,
+    DAG (Edge k) ->
+    Edge k (x,y) ->
+    DAG (Edge (join x y k)).
+  Proof.
+    intros.
+    unfold join.
+    assert (x <> y). {
+      unfold not; intros; subst.
+      assert (n: Reaches (Edge k) y y) by auto using edge_to_reaches.
+      apply H in n.
+      contradiction.
+    }
+    apply dag_join_aux_0; auto using incl_refl.
+  Qed.
+
+  Lemma eval_preserves_dag:
+    forall k o,
+    Check k o ->
+    DAG (Edge k) ->
+    DAG (Edge (eval o k)).
+  Proof.
+    intros.
+    destruct o; auto.
+    inversion H; subst; simpl; eauto.
+  Qed.
+
+  (**
+    If the safe-joins graph that yields a trace is well-formed, then
+    the safe-joins graph is a DAG.
+    *)
+
+  Theorem safe_to_dag:
+    forall t k,
+    Safe t k ->
+    DAG (Edge k).
+  Proof.
+    intros.
+    induction H. {
+      auto using f_dag_nil.
+    }
+    auto using eval_preserves_dag.
+  Qed.
+
+  Notation R_Edge rs k := (Edge (restriction tid_eq_dec rs k)).
+
+  Notation R_DAG rs k := (DAG (R_Edge rs k)).
+
+  Import WellFormed.
+
+  Let running_infimum:
+    forall rs k,
+    restriction tid_eq_dec rs k <> nil ->
+    R_DAG rs k ->
+    exists x, Graph.In (R_Edge rs k) x /\
+      forall y, ~ Reaches (R_Edge rs k) x y.
+  Proof.
+    intros.
+    apply dag_infimum; auto using TID.eq_dec.
+  Qed.
+
+
+  Let safe_to_r_dag:
+    forall t k rs,
+    Safe t k ->
+    R_DAG rs k.
+  Proof.
+    intros.
+    apply safe_to_dag in H.
+    apply f_dag_incl with (es:=k); auto using restriction_incl.
+  Qed.
+
+  Let progress_0:
+    forall t k rs,
+    Safe t k ->
+    (restriction tid_eq_dec rs k) <> nil ->
+    exists x, List.In x rs /\ forall y, Edge k (x,y) -> ~ List.In y rs.
+  Proof.
+    intros.
+    assert (Hx:
+      exists x, Graph.In (R_Edge rs k) x /\
+      forall y, ~ Reaches (R_Edge rs k) x y). {
+        eapply running_infimum; eauto.
+    }
+    destruct Hx as (x, (Hin, Hy)).
+    exists x.
+    split; eauto using restriction_in_1.
+    unfold not;
+    intros y He Hx.
+    assert (Hz := Hy y); clear Hy.
+    contradiction Hz; clear Hz.
+    assert (List.In x rs). {
+      eauto using restriction_in_1.
+    }
+    assert (R_Edge rs k (x,y)). {
+      unfold Edge.
+      auto using restriction_in_2.
+    }
+    auto using edge_to_reaches.
+  Qed.
+
+  Theorem progress:
+    forall t k rs,
+    Safe t k ->
+    rs <> nil ->
+    exists x, List.In x rs /\ forall y, Edge k (x,y) -> ~ List.In y rs.
+  Proof.
+    intros.
+    remember (restriction tid_eq_dec rs k) as l.
+    destruct l. {
+      subst.
+      destruct rs. { contradiction H0; auto. }
+      exists t0.
+      assert (List.In t0 (t0::rs)) by auto using in_eq.
+      split. { auto. }
+      intros.
+      unfold not; intros.
+      assert (List.In (t0, y) (restriction tid_eq_dec (t0::rs) k)) by auto using restriction_in_2.
+      rewrite <- Heql in *.
+      inversion H4.
+    }
+    assert (restriction tid_eq_dec rs k <> nil). {
+      intuition.
+      rewrite H1 in *.
+      inversion Heql.
+    }
+    eauto.
+  Qed.
+(*
+  Let sj_hb:
+    forall t x y z a k cg,
+    Safe t k ->
+    CG a t cg ->
+    List.In (Node.node_task x, Node.node_task z) k ->
+    HB_Edge cg (x, y) ->
+    List.In (Node.node_task y, Node.node_task z) k.
+  Proof.
+    intros.
+  Qed.
+
+  Let sj_hb_fork:
+    forall w a b x y z r k cg t,
+    a <> b ->
+    ~ Graph.In (Edge k) b ->
+    Safe (Some {| op_t := FORK; op_src := a; op_dst := b |} :: t) k ->
+    List.In (Node.node_task x, Node.node_task z) k ->
+    CG r (Some {| op_t := FORK; op_src := a; op_dst := b |} :: t) cg ->
+    Walk2 (HB_Edge cg) x y w ->
+    List.In (Node.node_task y, Node.node_task z) k.
+  Proof.
+    induction w; intros. {
+      apply walk2_nil_inv in H4; contradiction.
+    }
+    destruct a as (v1,v2).
+    assert (v1 = x) by eauto using walk2_inv_eq_fst; subst.
+    assert (HB_Edge cg (x,v2)). {
+      eapply walk2_to_edge; eauto using in_eq.
+    }
+    remember (Node.node_task y) as t_y.
+    remember (Node.node_task z) as t_z.
+    remember (Node.node_task x) as t_x.
+    unfold fork.
+    rewrite in_app_iff.
+    destruct (tid_eq_dec t_y a), (tid_eq_dec t_z b); subst.
+    - rewrite e; rewrite e0 in *.
+      eauto using in_eq.
+    - rewrite e in *.
+      right.
+      apply in_cons.
+      inversion H3; subst.
+  Qed.
+
+
+  Let sj_hb:
+    forall t x y z a k cg,
+    Safe t k ->
+    CG a t cg ->
+    List.In (Node.node_task x, Node.node_task z) k ->
+    HB cg x y ->
+    List.In (Node.node_task y, Node.node_task z) k.
+  Proof.
+    induction t; intros; simpl in *. {
+      inversion H0; subst; simpl in *.
+      apply hb_make_cg_absurd in H2; contradiction.
+    }
+    inversion H; subst.
+    inversion H0; subst.
+    inversion H5; subst; simpl in *.
+    - rename x0 into a; rename y0 into b.
+      rename cg0 into cg.
+      rename k0 into k.
+      clear H5.
+      assert (List.In (Node.node_task y, Node.node_task z) (fork a b k)). {
+        eapply IHt; eauto.
+      }
+subst.
+    destruct a0 as [(ot,os,od)|?].
+    - destruct ot; simpl in *.
+      + remember (Node.node_task x) as tx.
+        remember (Node.node_task y) as ty.
+        remember (Node.node_task z) as tz.
+      destruct (tid_eq_dec os x), (tid_eq_dec od z)
+  Qed.
+*)
+End Defs.
+
+Module Lang.
+
+  Fixpoint from_trace ts := 
+  match ts with
+  | nil => nil
+  | o :: ts => eval o (from_trace ts)
+  end.
+
+  Definition effects_to_sj ts := from_trace (CG.Lang.from_effects ts).
+
+  Definition Safe ts := Safe (CG.Lang.from_effects ts) (effects_to_sj ts).
+End Lang.
